raw_data_item_match, read_valid_cbor_from_buffer

src/cbor/CBOR.SteelC.fst
@@ -6,14 +6,23 @@ module C = Steel.ST.C.Types
 module U64 = FStar.UInt64
 module U8 = FStar.UInt8
 module SZ = FStar.SizeT
+module LPA = LowParse.SteelST.ArrayPtr
+module LPS = LowParse.SteelST.Parse
 
 noextract
 inline_for_extraction
 [@@ F.norm_field_attr]
 let cbor_string_fields =
   F.field_description_cons "byte_length" (C.scalar U64.t) (
-  F.field_description_cons "payload" (C.scalar (C.array (C.scalar U8.t)))
-  F.field_description_nil)
+  F.field_description_cons "payload" (C.scalar LPS.byte_array) (
+  F.field_description_nil
+))
+
+noextract inline_for_extraction [@@ F.norm_field_attr]
+let cbor_string_byte_length : F.field_t cbor_string_fields = "byte_length"
+
+noextract inline_for_extraction [@@ F.norm_field_attr]
+let cbor_string_payload : F.field_t cbor_string_fields = "payload"
 
 let cbor_string = C.struct_t "" cbor_string_fields
 
@@ -25,8 +34,15 @@ inline_for_extraction
 [@@ F.norm_field_attr]
 let cbor_serialized_fields =
   F.field_description_cons "byte_size" (C.scalar SZ.t) (
-  F.field_description_cons "payload" (C.scalar (C.array (C.scalar U8.t)))
-  F.field_description_nil)
+  F.field_description_cons "payload" (C.scalar LPS.byte_array) (
+  F.field_description_nil
+))
+
+noextract inline_for_extraction [@@ F.norm_field_attr]
+let cbor_serialized_byte_size : F.field_t cbor_serialized_fields = "byte_size"
+
+noextract inline_for_extraction [@@ F.norm_field_attr]
+let cbor_serialized_payload : F.field_t cbor_serialized_fields = "payload"
 
 let cbor_serialized = C.struct_t "" cbor_serialized_fields
 
@@ -42,6 +58,12 @@ let cbor_tagged_fields =
   F.field_description_nil
 ))
 
+noextract inline_for_extraction [@@ F.norm_field_attr]
+let cbor_tagged_tag : F.field_t cbor_tagged_fields = "tag"
+
+noextract inline_for_extraction [@@ F.norm_field_attr]
+let cbor_tagged_payload : F.field_t cbor_tagged_fields = "payload"
+
 let cbor_tagged = C.struct_t "" cbor_tagged_fields
 
 noextract
@@ -56,6 +78,12 @@ let cbor_array_fields =
   F.field_description_nil
 ))
 
+noextract inline_for_extraction [@@ F.norm_field_attr]
+let cbor_array_count : F.field_t cbor_array_fields = "count"
+
+noextract inline_for_extraction [@@ F.norm_field_attr]
+let cbor_array_payload : F.field_t cbor_array_fields = "payload"
+
 let cbor_array = C.struct_t "" cbor_array_fields
 
 noextract
@@ -66,9 +94,15 @@ inline_for_extraction
 [@@ F.norm_field_attr]
 let cbor_map_fields =
   F.field_description_cons "entry_count" (C.scalar U64.t) (
-  F.field_description_cons "payload" (C.scalar C.void_ptr) (
+  F.field_description_cons "payload" (C.scalar C.array_void_ptr) (
   F.field_description_nil
 ))
+
+noextract inline_for_extraction [@@ F.norm_field_attr]
+let cbor_map_entry_count : F.field_t cbor_map_fields = "entry_count"
+
+noextract inline_for_extraction [@@ F.norm_field_attr]
+let cbor_map_payload : F.field_t cbor_map_fields = "payload"
 
 let cbor_map = C.struct_t "" cbor_map_fields
 
@@ -89,19 +123,57 @@ let cbor_case_fields =
   F.field_description_nil
 )))))))
 
+noextract inline_for_extraction [@@ F.norm_field_attr]
+let cbor_case_int64 : F.field_t cbor_case_fields = "case_int64"
+
+noextract inline_for_extraction [@@ F.norm_field_attr]
+let cbor_case_string : F.field_t cbor_case_fields = "case_string"
+
+noextract inline_for_extraction [@@ F.norm_field_attr]
+let cbor_case_tagged : F.field_t cbor_case_fields = "case_tagged"
+
+noextract inline_for_extraction [@@ F.norm_field_attr]
+let cbor_case_array : F.field_t cbor_case_fields = "case_array"
+
+noextract inline_for_extraction [@@ F.norm_field_attr]
+let cbor_case_map : F.field_t cbor_case_fields = "case_map"
+
+noextract inline_for_extraction [@@ F.norm_field_attr]
+let cbor_case_simple_value : F.field_t cbor_case_fields = "case_simple_value"
+
+noextract inline_for_extraction [@@ F.norm_field_attr]
+let cbor_case_serialized : F.field_t cbor_case_fields = "case_serialized"
+
 let cbor_case = C.union_t "" cbor_case_fields
 
 noextract
 let cbor_case_td : C.typedef cbor_case = C.union0 _ _ _
 
+[@@CMacro]
+let cbor_type_serialized = 255uy
+
+let cbor_type_prop
+  (x: U8.t)
+: Tot prop
+= U8.v x < pow2 3 \/
+  x == cbor_type_serialized
+
+let cbor_type_t = (x: U8.t { cbor_type_prop x })
+
 noextract
 inline_for_extraction
 [@@ F.norm_field_attr]
 let cbor_fields =
-  F.field_description_cons "type" (C.scalar Cbor.major_type_t) (
+  F.field_description_cons "type" (C.scalar cbor_type_t) (
   F.field_description_cons "payload" cbor_case_td (
   F.field_description_nil
 ))
+
+noextract inline_for_extraction [@@ F.norm_field_attr]
+let cbor_type : F.field_t cbor_fields = "type"
+
+noextract inline_for_extraction [@@ F.norm_field_attr]
+let cbor_payload : F.field_t cbor_fields = "payload"
 
 let cbor = C.struct_t "" cbor_fields
 
@@ -117,6 +189,12 @@ let cbor_pair_fields =
   F.field_description_nil
 ))
 
+noextract inline_for_extraction [@@ F.norm_field_attr]
+let cbor_pair_fst : F.field_t cbor_pair_fields = "fst"
+
+noextract inline_for_extraction [@@ F.norm_field_attr]
+let cbor_pair_snd : F.field_t cbor_pair_fields = "snd"
+
 let cbor_pair = C.struct_t "" cbor_pair_fields
 
 noextract
@@ -124,22 +202,337 @@ let cbor_pair_td : C.typedef cbor_pair = C.struct0 _ _ _
 
 open Steel.ST.Util
 
-#set-options "--print_implicits"
-
 let test (#s: Ghost.erased cbor_case) (p: C.ref cbor_case_td)
 : ST (Ghost.erased cbor_case)
     (C.pts_to p s)
     (fun s' -> C.pts_to p s')
     (C.full cbor_case_td s)
     (fun s' -> C.full cbor_case_td s')
-= let ps = C.union_switch_field0 _ p "case_int64" (C.scalar U64.t) in
+= let ps = C.union_switch_field0 _ p cbor_case_int64 (C.scalar U64.t) in
   C.write ps 1729uL;
-  let _ = C.ununion_field p "case_int64" ps in
-  drop (C.has_union_field p "case_int64" _);
-  let ps = C.union_field0 _ p "case_int64" (C.scalar U64.t) in
+  let _ = C.ununion_field p cbor_case_int64 ps in
+  drop (C.has_union_field p cbor_case_int64 _);
+  let ps = C.union_field0 _ p cbor_case_int64 (C.scalar U64.t) in
   C.write ps 42uL;
-  let _ = C.ununion_field p "case_int64" ps in
-  drop (C.has_union_field p "case_int64" _);
+  let _ = C.ununion_field p cbor_case_int64 ps in
+  drop (C.has_union_field p cbor_case_int64 _);
   let s' = vpattern_replace (C.pts_to p) in
-  C.full_union (Ghost.reveal s') "case_int64"; // FIXME: find a better pattern for that lemma
+  C.full_union (Ghost.reveal s') cbor_case_int64; // FIXME: find a better pattern for that lemma
   return _
+
+let raw_data_item_match_serialized_prop
+  (c: cbor)
+  (v: Cbor.raw_data_item)
+  (a: LPS.byte_array)
+  (w: LPS.v Cbor.parse_raw_data_item_kind Cbor.raw_data_item)
+: GTot prop
+= let payload = C.struct_get_field c cbor_payload in
+  C.struct_get_field c cbor_type == C.mk_scalar cbor_type_serialized /\
+  C.union_get_case payload == Some cbor_case_serialized /\
+  begin let payload = C.union_get_field payload cbor_case_serialized in
+    C.struct_get_field payload cbor_serialized_byte_size == C.mk_scalar (LPA.len (LPS.array_of w)) /\
+    w.contents == v /\
+    C.struct_get_field payload cbor_serialized_payload == C.mk_scalar a
+  end
+
+[@@__reduce__]
+let raw_data_item_match_serialized0
+  (c: cbor)
+  (v: Cbor.raw_data_item)
+: Tot vprop
+= exists_ (fun (a: LPS.byte_array) -> exists_ (fun (w: LPS.v Cbor.parse_raw_data_item_kind Cbor.raw_data_item) ->
+    LPS.aparse Cbor.parse_raw_data_item a w `star`
+    pure (
+      raw_data_item_match_serialized_prop c v a w
+    )
+  ))
+
+let raw_data_item_match_simple_value_prop
+  (c: cbor)
+  (v: Cbor.raw_data_item { Cbor.Simple? v })
+: GTot prop
+= let Cbor.Simple v = v in
+  let payload = C.struct_get_field c cbor_payload in
+  C.struct_get_field c cbor_type == C.mk_scalar Cbor.major_type_simple_value /\
+  C.union_get_case payload == Some cbor_case_simple_value /\
+  C.union_get_field payload cbor_case_simple_value == C.mk_scalar v
+
+[@@__reduce__]
+let raw_data_item_match_simple_value0
+  (c: cbor)
+  (v: Cbor.raw_data_item { Cbor.Simple? v })
+: Tot vprop
+= pure (raw_data_item_match_simple_value_prop c v)
+
+let raw_data_item_match_int64_prop
+  (c: cbor)
+  (v: Cbor.raw_data_item { Cbor.Int64? v })
+: GTot prop
+= let Cbor.Int64 ty v = v in
+  let payload = C.struct_get_field c cbor_payload in
+  C.struct_get_field c cbor_type == C.mk_scalar ty /\
+  C.union_get_case payload == Some cbor_case_int64 /\
+  C.union_get_field payload cbor_case_int64 == C.mk_scalar v
+
+[@@__reduce__]
+let raw_data_item_match_int64_0
+  (c: cbor)
+  (v: Cbor.raw_data_item { Cbor.Int64? v })
+: Tot vprop
+= pure (raw_data_item_match_int64_prop c v)
+
+module U64 = FStar.UInt64
+
+let raw_data_item_match_string_prop
+  (c: cbor)
+  (v: Cbor.raw_data_item { Cbor.String? v })
+  (a: LPS.byte_array)
+  (w: LPA.v U8.t)
+: GTot prop
+= let Cbor.String ty s = v in
+  let payload = C.struct_get_field c cbor_payload in
+  C.struct_get_field c cbor_type == C.mk_scalar ty /\
+  C.union_get_case payload == Some cbor_case_string /\
+  begin let payload = C.union_get_field payload cbor_case_string in
+    C.struct_get_field payload cbor_string_byte_length == C.mk_scalar (U64.uint_to_t (Seq.length s)) /\
+    LPA.contents_of w == s /\
+    C.struct_get_field payload cbor_string_payload == C.mk_scalar a
+  end
+
+[@@__reduce__]
+let raw_data_item_match_string0
+  (c: cbor)
+  (v: Cbor.raw_data_item { Cbor.String? v })
+: Tot vprop
+= exists_ (fun (a: LPS.byte_array) -> exists_ (fun (w: LPA.v U8.t) ->
+    LPA.arrayptr a w `star`
+    pure (
+      raw_data_item_match_string_prop c v a w
+    )
+  ))
+
+let raw_data_item_match_tagged_prop
+  (c: cbor)
+  (v: Cbor.raw_data_item { Cbor.Tagged? v })
+  (a: C.ref cbor_td)
+: GTot prop
+= let Cbor.Tagged tag v = v in
+  let payload = C.struct_get_field c cbor_payload in
+  C.struct_get_field c cbor_type == C.mk_scalar Cbor.major_type_tagged /\
+  C.union_get_case payload == Some cbor_case_tagged /\
+  begin let payload = C.union_get_field payload cbor_case_tagged in
+    C.struct_get_field payload cbor_tagged_tag == C.mk_scalar tag /\
+    C.struct_get_field payload cbor_tagged_payload == C.mk_scalar a
+  end
+
+[@@__reduce__]
+let raw_data_item_match_tagged0
+  (c: cbor)
+  (v: Cbor.raw_data_item { Cbor.Tagged? v })
+  (raw_data_item_match: (cbor -> (v': Cbor.raw_data_item { v' << v }) -> vprop))
+: Tot vprop
+= exists_ (fun (a: C.ref cbor_td) -> exists_ (fun (c': Ghost.erased cbor) ->
+    C.pts_to a c' `star`
+    raw_data_item_match c' (Cbor.Tagged?.v v) `star`
+    pure (
+      raw_data_item_match_tagged_prop c v a
+    )
+  ))
+
+let raw_data_item_match_array_prop
+  (c: cbor)
+  (v: Cbor.raw_data_item { Cbor.Array? v })
+  (a: C.array_ptr cbor_td)
+: GTot prop
+= let Cbor.Array l = v in
+  let payload = C.struct_get_field c cbor_payload in
+  C.struct_get_field c cbor_type == C.mk_scalar Cbor.major_type_array /\
+  C.union_get_case payload == Some cbor_case_array /\
+  begin let payload = C.union_get_field payload cbor_case_array in
+    C.struct_get_field payload cbor_array_count == C.mk_scalar (U64.uint_to_t (List.Tot.length l)) /\
+    C.struct_get_field payload cbor_array_payload == C.mk_scalar a
+  end
+
+[@@__reduce__]
+let raw_data_item_match_array0
+  (c: cbor)
+  (v: Cbor.raw_data_item { Cbor.Array? v })
+  (raw_data_item_array_match: (Seq.seq cbor -> (v': list Cbor.raw_data_item { v' << v }) -> vprop))
+: Tot vprop
+= exists_ (fun (a: C.array cbor_td) -> exists_ (fun (c': Ghost.erased (Seq.seq cbor)) ->
+    C.array_pts_to a c' `star`
+    raw_data_item_array_match c' (Cbor.Array?.v v) `star`
+    pure (
+      raw_data_item_match_array_prop c v (C.array_ptr_of a)
+    )
+  ))
+
+let raw_data_item_match_map_prop
+  (c: cbor)
+  (v: Cbor.raw_data_item { Cbor.Map? v })
+  (a: C.array_ptr cbor_pair_td)
+: GTot prop
+= let Cbor.Map l = v in
+  let payload = C.struct_get_field c cbor_payload in
+  C.struct_get_field c cbor_type == C.mk_scalar Cbor.major_type_map /\
+  C.union_get_case payload == Some cbor_case_map /\
+  begin let payload = C.union_get_field payload cbor_case_map in
+    C.struct_get_field payload cbor_map_entry_count == C.mk_scalar (U64.uint_to_t (List.Tot.length l)) /\
+    C.struct_get_field payload cbor_map_payload == C.mk_scalar a
+  end
+
+[@@__reduce__]
+let raw_data_item_match_map0
+  (c: cbor)
+  (v: Cbor.raw_data_item { Cbor.Map? v })
+  (raw_data_item_map_match: (Seq.seq cbor_pair -> (v': list (Cbor.raw_data_item & Cbor.raw_data_item) { v' << v }) -> vprop))
+: Tot vprop
+= exists_ (fun (a: C.array cbor_pair_td) -> exists_ (fun (c': Ghost.erased (Seq.seq cbor_pair)) ->
+    C.array_pts_to a c' `star`
+    raw_data_item_map_match c' (Cbor.Map?.v v) `star`
+    pure (
+      raw_data_item_match_map_prop c v (C.array_ptr_of a)
+    )
+  ))
+
+[@@__reduce__]
+let raw_data_item_array_match_nil0
+  (c: Seq.seq cbor)
+: Tot vprop
+= pure (c `Seq.equal` Seq.empty)
+
+[@@__reduce__]
+let raw_data_item_array_match_cons0
+  (c: Seq.seq cbor)
+  (l: list Cbor.raw_data_item { Cons? l })
+  (raw_data_item_match: (cbor -> (v': Cbor.raw_data_item { v' << l }) -> vprop))
+  (raw_data_item_array_match: (Seq.seq cbor -> (v': list Cbor.raw_data_item { v' << l }) -> vprop))
+: Tot vprop
+= exists_ (fun (c1: cbor) -> exists_ (fun (c2: Seq.seq cbor) ->
+    raw_data_item_match c1 (List.Tot.hd l) `star`
+    raw_data_item_array_match c2 (List.Tot.tl l) `star`
+    pure (c `Seq.equal` Seq.cons c1 c2)
+  ))
+
+[@@__reduce__]
+let raw_data_item_map_match_nil0
+  (c: Seq.seq cbor_pair)
+: Tot vprop
+= pure (c `Seq.equal` Seq.empty)
+
+noextract
+let fstp (#a1 #a2: Type) (x: (a1 & a2)) : Tot a1 = fst x
+
+noextract
+let sndp (#a1 #a2: Type) (x: (a1 & a2)) : Tot a2 = snd x
+
+[@@__reduce__]
+let raw_data_item_map_match_cons0
+  (c: Seq.seq cbor_pair)
+  (l: list (Cbor.raw_data_item & Cbor.raw_data_item) { Cons? l })
+  (raw_data_item_match: (cbor -> (v': Cbor.raw_data_item { v' << l }) -> vprop))
+  (raw_data_item_map_match: (Seq.seq cbor_pair -> (v': list (Cbor.raw_data_item & Cbor.raw_data_item) { v' << l }) -> vprop))
+: Tot vprop
+= exists_ (fun (c1: cbor_pair) -> exists_ (fun (c2: Seq.seq cbor_pair) ->
+    raw_data_item_match (C.struct_get_field c1 cbor_pair_fst) (fstp (List.Tot.hd l)) `star`
+    raw_data_item_match (C.struct_get_field c1 cbor_pair_snd) (sndp (List.Tot.hd l)) `star`
+    raw_data_item_map_match c2 (List.Tot.tl l) `star`
+    pure (c `Seq.equal` Seq.cons c1 c2)
+  ))
+
+let rec raw_data_item_match0
+  (c: cbor)
+  (v: Cbor.raw_data_item)
+: Tot vprop
+  (decreases v)
+= if C.get_scalar_value (C.struct_get_field c cbor_type) = Some cbor_type_serialized
+  then raw_data_item_match_serialized0 c v
+  else match v with
+  | Cbor.Simple _ -> raw_data_item_match_simple_value0 c v
+  | Cbor.Int64 _ _ -> raw_data_item_match_int64_0 c v
+  | Cbor.String _ _ -> raw_data_item_match_string0 c v
+  | Cbor.Array _ -> raw_data_item_match_array0 c v raw_data_item_array_match0
+  | Cbor.Map _ -> raw_data_item_match_map0 c v raw_data_item_map_match0
+  | Cbor.Tagged _ _ -> raw_data_item_match_tagged0 c v raw_data_item_match0
+
+and raw_data_item_array_match0
+  (c: Seq.seq cbor)
+  (v: list Cbor.raw_data_item)
+: Tot vprop
+  (decreases v)
+= match v with
+  | [] -> raw_data_item_array_match_nil0 c
+  | _ :: _ -> raw_data_item_array_match_cons0 c v raw_data_item_match0 raw_data_item_array_match0
+
+and raw_data_item_map_match0
+  (c: Seq.seq cbor_pair)
+  (v: list (Cbor.raw_data_item & Cbor.raw_data_item))
+: Tot vprop
+  (decreases v)
+= match v with
+  | [] -> raw_data_item_map_match_nil0 c
+  | _ :: _ -> raw_data_item_map_match_cons0 c v raw_data_item_match0 raw_data_item_map_match0
+
+irreducible
+let raw_data_item_match : (phi: (
+  (c: cbor) ->
+  (v: Cbor.raw_data_item) ->
+  Tot vprop
+) {phi == raw_data_item_match0}
+) = raw_data_item_match0
+
+let raw_data_item_match_eq : squash (raw_data_item_match == raw_data_item_match0) = ()
+
+let raw_data_item_match_intro_serialized
+  (#opened: _)
+  (c: Ghost.erased cbor)
+  (v: Cbor.raw_data_item)
+  (a: LPS.byte_array)
+  (w: LPS.v Cbor.parse_raw_data_item_kind Cbor.raw_data_item)
+: STGhost unit opened
+    (LPS.aparse Cbor.parse_raw_data_item a w)
+    (fun _ -> raw_data_item_match (Ghost.reveal c) v)
+    (raw_data_item_match_serialized_prop (Ghost.reveal c) v a w)
+    (fun _ -> True)
+= noop ();
+  rewrite
+    (raw_data_item_match_serialized0 c v)
+    (raw_data_item_match c v)
+
+#restart-solver
+
+let read_valid_cbor_from_buffer
+  (#va: LPS.v Cbor.parse_raw_data_item_kind Cbor.raw_data_item)
+  (#c: Ghost.erased cbor)
+  (a: LPS.byte_array)
+  (alen: SZ.t)
+  (tgt: C.ref cbor_td)
+: ST (Ghost.erased cbor)
+    (LPS.aparse Cbor.parse_raw_data_item a va `star`
+      C.pts_to tgt c
+    )
+    (fun c' ->
+      C.pts_to tgt c'
+      `star` raw_data_item_match (Ghost.reveal c') va.contents
+    )
+    (alen == LPA.len (LPS.array_of va) /\
+      C.full cbor_td c
+    )
+    (fun _ -> True)
+=
+  let ptype = C.struct_field1 _ tgt cbor_type (C.scalar cbor_type_t) (_ by (F.norm_fields ())) (_ by (F.norm_fields ())) in
+  C.write ptype cbor_type_serialized;
+  let _ = C.unstruct_field_and_drop tgt cbor_type ptype in
+  let payload1 = C.struct_field1 _ tgt cbor_payload cbor_case_td (_ by (F.norm_fields ())) (_ by (F.norm_fields ())) in
+  let payload2 = C.union_switch_field1 _ payload1 cbor_case_serialized cbor_serialized_td (_ by (F.norm_fields ())) (_ by (F.norm_fields ())) in
+  let plen = C.struct_field1 _ payload2 cbor_serialized_byte_size (C.scalar SZ.t) (_ by (F.norm_fields ())) (_ by (F.norm_fields ())) in
+  C.write plen alen;
+  let _ = C.unstruct_field_and_drop payload2 cbor_serialized_byte_size plen in
+  let payload3 = C.struct_field1 _ payload2 cbor_serialized_payload (C.scalar LPS.byte_array) (_ by (F.norm_fields ())) (_ by (F.norm_fields ())) in
+  C.write payload3 a;
+  let _ = C.unstruct_field_and_drop payload2 cbor_serialized_payload payload3 in
+  let _ = C.ununion_field_and_drop payload1 cbor_case_serialized payload2 in
+  let _ = C.unstruct_field_and_drop tgt cbor_payload payload1 in
+  let c' = vpattern_replace (C.pts_to tgt) in
+  raw_data_item_match_intro_serialized c' va.contents a va;
+  return c'
